<?xml version="1.0" encoding="UTF-8"?>
<rdf:RDF
	xmlns:rdf="http://www.w3.org/1999/02/22-rdf-syntax-ns#"
	xmlns:owl="http://www.w3.org/2002/07/owl#"
	xmlns:rdfs="http://www.w3.org/2000/01/rdf-schema#"
	xmlns:math="http://numerateweb.org/vocab/math#"
	xmlns:xsd="http://www.w3.org/2001/XMLSchema#"
	xml:base="http://numerateweb.org/vocab/math/meta">
<rdf:Description rdf:about="http://numerateweb.org/vocab/math#Symbol">
	<rdfs:subClassOf>
		<owl:Restriction rdf:nodeID="node17tt88171x1">
			<owl:allValuesFrom rdf:resource="http://numerateweb.org/vocab/math#Object"/>
			<owl:onProperty rdf:resource="#example"/>
		</owl:Restriction>
	</rdfs:subClassOf>
	<rdfs:subClassOf>
		<owl:Restriction rdf:nodeID="node17tt88171x2">
			<owl:allValuesFrom rdf:resource="http://numerateweb.org/vocab/math#Object"/>
			<owl:onProperty rdf:resource="#formalProperty"/>
		</owl:Restriction>
	</rdfs:subClassOf>
	<rdfs:subClassOf>
		<owl:Restriction rdf:nodeID="node17tt88171x3">
			<owl:allValuesFrom rdf:resource="#Library"/>
			<owl:onProperty rdf:resource="http://www.w3.org/2000/01/rdf-schema#isDefinedBy"/>
		</owl:Restriction>
	</rdfs:subClassOf>
</rdf:Description>
<owl:Ontology rdf:about="">
	<owl:imports rdf:resource="http://numerateweb.org/vocab/math"/>
</owl:Ontology>
<owl:Class rdf:about="#ApplicationSymbol">
	<rdfs:comment>The symbol may appear as the first child of an OpenMath application object.  </rdfs:comment>
	<rdfs:subClassOf rdf:resource="http://numerateweb.org/vocab/math#Symbol"/>
</owl:Class>
<owl:Class rdf:about="#AttributionSymbol">
	<rdfs:comment>The symbol may be used as key in an OpenMath attribution object, i.e. as the first element of a (key, value) pair, or in an equivalent context (for example to refer to the value of an attribution).  This form of attribution
may be ignored by an application, so should be used for information which does not change the meaning of the attributed OpenMath object.</rdfs:comment>
	<rdfs:subClassOf rdf:resource="http://numerateweb.org/vocab/math#Symbol"/>
</owl:Class>
<owl:Class rdf:about="#BinderSymbol">
	<rdfs:comment>The symbol may appear as the first child of an OpenMath binding object.
</rdfs:comment>
	<rdfs:subClassOf rdf:resource="http://numerateweb.org/vocab/math#Symbol"/>
</owl:Class>
<owl:Class rdf:about="#ConstantSymbol">
	<rdfs:comment>The symbol cannot be used to construct an OpenMath compound object.
</rdfs:comment>
	<rdfs:subClassOf rdf:resource="http://numerateweb.org/vocab/math#Symbol"/>
</owl:Class>
<owl:Class rdf:about="#ErrorSymbol">
	<rdfs:comment>The symbol may appear as the first child of an OpenMath error object.</rdfs:comment>
	<rdfs:subClassOf rdf:resource="http://numerateweb.org/vocab/math#Symbol"/>
</owl:Class>
<owl:Class rdf:about="#Library">
	<rdfs:comment>Represents a collection of related OpenMath symbols.</rdfs:comment>
</owl:Class>
<owl:Class rdf:about="#SemanticAttributionSymbol">
	<rdfs:comment>This is the same as attribution except that it modifies the meaning of the attributed OpenMath object and thus cannot be ignored by an application, without changing the meaning.</rdfs:comment>
	<rdfs:subClassOf rdf:resource="http://numerateweb.org/vocab/math#Symbol"/>
</owl:Class>
<owl:DatatypeProperty rdf:about="#commentedProperty">
	<rdfs:subPropertyOf rdf:resource="http://www.w3.org/2002/07/owl#topDataProperty"/>
</owl:DatatypeProperty>
<owl:DatatypeProperty rdf:about="#description">
	<rdfs:subPropertyOf rdf:resource="http://www.w3.org/2002/07/owl#topDataProperty"/>
</owl:DatatypeProperty>
<owl:ObjectProperty rdf:about="#example">
	<rdfs:subPropertyOf rdf:resource="http://www.w3.org/2002/07/owl#topObjectProperty"/>
</owl:ObjectProperty>
<owl:ObjectProperty rdf:about="#formalProperty">
	<rdfs:subPropertyOf rdf:resource="http://www.w3.org/2002/07/owl#topObjectProperty"/>
</owl:ObjectProperty>

</rdf:RDF>